\input{../latex/header.tex}

\title{Homework 3: Exact Symplectic Manifolds}
\author{Yannis B\"ahni}
\address[Yannis B\"ahni]{University of Zurich, R\"amistrasse 71, 8006 Zurich}
\email[Yannis B\"ahni]{\href{mailto:yannis.baehni@uzh.ch}{yannis.baehni@uzh.ch}}

\begin{document}

\maketitle
\thispagestyle{fancy}
\setcounter{section}{1}

\begin{exercise}
Let $M$ and $N$ be smooth manifolds, $F : M \to N$ a diffeomorphism and $A \in \Gamma\del[1]{T^{(0,k)}TN}$, $k \in \Zbb$, $k \geq 1$. Then 
\begin{equation}
F^*A(X_1,\dots,X_k) = A(F_*X_1,\dots,F_*X_k) \circ F
\end{equation}
\noindent holds for all $X_1,\dots,X_k \in \Xfrak(M)$.
\label{ex_properties_pullback}
\end{exercise}

\begin{solution}
Let $p \in M$. Then
\begin{align*}
F^*A(X_1,\dots,X_k)(p) &= (F^*A)_p(X_1\vert_p,\dots,X_k\vert_p)\\
&= A_{F(p)}\del[1]{d F_p(X_1\vert_p),\dots,d F_p(X_k\vert_p)}\\
&= A_{F(p)}\del[1]{(F_*X_1)_{F(p)},\dots,(F_*X_k)_{F(p)}}\\
&= A\del[1]{F_*X_1,\dots,F_*X_k}\del[1]{F(p)}.
\end{align*}
\end{solution}

\begin{exercise} 
\begin{enumerate}[label = \textup{(}\alph*\textup{)}]
\item  
\end{enumerate}
\end{exercise}

\begin{solution}
	For (a), consider the tangent-cotangent isomorphism $\wtilde{\omega} : TM \to T^*M$. Set $X := \wtilde{\omega}^{-1}(-\alpha)$. As a composition of smooth functions, $X : M \to TM$ is smooth. Moreover, $X_p = \wtilde{\omega}^{-1}(-\alpha_p) \in T_pM$. Thus $X \in \Xfrak(M)$. Moreover 
	\begin{equation*}
		i_X \omega = \wtilde{\omega}\del[1]{\wtilde{\omega}^{-1}(-\alpha)} = - \alpha.  
	\end{equation*}
	Since $\wtilde{\omega}$ is an isomorphism, $X$ is unique. Cartan's magic formula together with the assumption $\omega = -d\alpha$ yields
	\begin{equation*}
		\Lcal_X \omega = di_X\omega + i_Xd\omega = di_X \omega = -d\alpha = \omega.
	\end{equation*}
	For proving (b), assume that $L_X \omega = \omega$ for some $X \in \Xfrak(M)$. Again, Cartan's magic formula yields
	\begin{equation*}
		\Lcal_X\omega = di_X\omega + i_Xd\omega = di_X\omega = \omega.
	\end{equation*}
	Now $i_X\omega \in \Omega^1(M)$ and thus $\omega$ is exact.\\
	For proving (c), an application of the Fisherman's formula yields 
	\begin{equation*}
		\frac{d}{dt} (\exp tX)^* \omega = (\exp tX)^* \Lcal_X \omega = (\exp tX)^* \omega
	\end{equation*}
	\noindent and the property of the flow $\exp tX$ yields
	\begin{equation*}
		(\exp tX\vert_0)^*\omega = \id_M^* \omega = \omega.
	\end{equation*}
	Also we have that $\frac{d}{dt}e^t\omega = e^t\omega$ and $e^0\omega = \omega$. Hence $(\exp tX)^* \omega$ and $e^t\omega$ solve the same locally uniquely solvable initial value problem and are therefore locally equal.\\
	For proving (d), observe that for $Y \in \Xfrak(M)$ we have that
	\begin{align*}
		\omega(g_*X,Y) \circ g &= (g^*\omega)(X,g_*^{-1}Y)\\
		&= \omega\del[1]{X,g_*^{-1}Y}\\
		&= i_X\omega\del[1]{g_*^{-1}Y}\\
		&= -\alpha\del[1]{g_*^{-1}Y} \circ g^{-1}\\
		&= -(g^*\alpha)\del[1]{g_*^{-1}Y}\\
		&= -\alpha(Y) \circ g\\
		&= i_X\omega(Y) \circ g\\
		&= \omega(X,Y) \circ g.
	\end{align*}
	Thus $\wtilde{\omega}(g_*X) = \wtilde{\omega}(X)$ and since $\wtilde{\omega}$ is an isomorphism, we have that $g_*X = X$.\\
	For proving (e), let us define $\rho_t := g \circ \exp tX \circ g^{-1}$. Then 
	\begin{equation*}
		\rho_0 = g \circ \exp tX \vert_{t = 0} \circ g^{-1} = \id_M
	\end{equation*}
	\noindent and
	\begin{align*}
		\frac{d}{dt} \rho_t(p) &= \frac{d}{dt}g\del[1]{\exp tX\del[1]{g^{-1}(p)}}\\
		&= dg_{\exp tX\del[0]{g^{-1}(p)}}\frac{d}{dt}\exp tX\del[1]{g^{-1}(p)}\\
		&= dg_{\exp tX\del[0]{g^{-1}(p)}}X\del[1]{\exp tX\del[1]{g^{-1}(p)}}\\
		&= (g_*X)_{(g \circ \exp tX \circ g^{-1})(p)}.
	\end{align*}
	Thus $\rho_t$ is the flow of the vector field $g_* X$. By part (d) $g_* X$ coincides with $X$ and thus $\rho_t$ is also the flow of $X$. But flows are unique and thus 
	\begin{equation*}
		g \circ \exp tX \circ g^{-1} = \exp tX
	\end{equation*}
	\noindent from which the claim follows.\\
	For (f), let us compute $\Lcal_X \omega_0$. We have
	\begin{align*}
		\Lcal_X\omega_0 &= di_X\omega_0\\
		&= d \sum_{i = 1}^n \del[1]{(i_X dx_i) \wedge dy_i - dx_i \wedge (i_Xdy_i)}\\
		&= \frac{1}{2}d \sum_{i = 1}^n (x_i dy_i - y_idx_i)\\
		&= \frac{1}{2}\sum_{i = 1}^n (dx_i \wedge dy_i - dy_i \wedge dx_i)\\
		&= \omega_0.
	\end{align*}
\end{solution}

\begin{exercise} 
\begin{enumerate}[label = \textup{(}\alph*\textup{)}]
\item  
\end{enumerate}
\end{exercise}

\begin{solution}
	For showing (a), let us consider $X := f^i \frac{\partial}{\partial x^i} + g^i \frac{\partial}{\partial \xi^i}$. Then
	\begin{align*}
		i_X\omega &= i_X\sum_{i = 1}^n dx_i \wedge d\xi_i\\
		&= \sum_{i = 1}^n \del[1]{(i_Xdx_i) \wedge d\xi_i - dx_i \wedge (i_X d\xi_i)}\\
		&= \sum_{i = 1}^n \del[1]{f^i d\xi_i - g^i dx_i}. 
	\end{align*}
	Comparing this with $-\alpha$ yields $f^i = 0$ and $g^i = \xi^i$ for all $i = 1,\dots,n$. Hence
	\begin{equation*}
		X = \xi^i \frac{\partial}{\partial \xi^i}.
	\end{equation*}
\end{solution}

\appendix
\begin{appendix}
	\section{The Tubular Neighbourhood Theorem}
	\begin{theorem}[Generalization of the Inverse Function Theorem]
		Let $M$ and $N$ be smooth manifolds and $S$ a compact immersed submanifold of $M$. Moreover, let $f : M \to N$ be smooth such that $f\vert_S$ is injective. Suppose that $df_p$ is an isomorphism for all $x \in S$.
	\end{theorem}
\end{appendix}

\end{document}
