\input{header.tex}

\title{Solutions Sheet 8}
\author{Yannis B\"{a}hni}
\address[Yannis B\"{a}hni]{University of Zurich, R\"{a}mistrasse 71, 8006 Zurich}
\email[Yannis B\"{a}hni]{\href{mailto:yannis.baehni@uzh.ch}{\nolinkurl{yannis.baehni@uzh.ch}}}

\begin{document}

\maketitle
\thispagestyle{fancy}

\setcounter{section}{1}

\begin{enumerate}[label = \textbf{Exercise \arabic*.},wide = 0pt, itemsep = 1.5ex]
	\item
	\item We will show that there exists a unique solution to the integral equation $f \in L^2(X)$. 
		\begin{lemma}
			Let $L \in L^2(X \times X)$ and $f \in L^2(X)$. For $x \in X$ define
			\begin{equation*}
				g_f(x) := \int_X L(x,y)f(y)dy.
			\end{equation*}
			Then $g_f \in L^2(X)$.
			\label{lem:L^2}
		\end{lemma}

		\begin{proof}
			We have that
			\begin{align*}
				\norm[0]{g_f}_{L^2(X)}^2 &= \int_X \abs[0]{g_f(x)}^2 dx\\
				&= \int_X \abs[3]{\int_X L(x,y)f(y)dy}^2 dx\\
				&\leq \int_X \del[3]{\int_X \abs{L(x,y)f(y)}dy}^2 dx\\
				&= \int_X \norm[0]{L(x,\cdot)f}_{L^1(X)}^2 dx\\
			&\leq \int_X \norm[0]{L(x,\cdot)}_{L^2(X)}^2 \norm[0]{f}_{L^2(X)}^2 dx\\
			&= \norm[0]{f}_{L^2(X)}^2 \int_X \int_X \abs[0]{L(x,y)}^2dy dx\\
			&= \norm[0]{f}_{L^2(X)}^2 \norm[0]{L}_{L^2(X \times X)}^2
			\end{align*}
		\noindent by H\"older and Fubini.
		\end{proof}
		Now we have to solve the equation
		\begin{equation*}
			cf + u = g_f.
		\end{equation*}
		Define $a : L^2(X) \times L^2(X) \to \mathbb{C}$ by
		\begin{equation*}
			a(f,\varphi) := \langle cf - g_f, \varphi \rangle_{L^2(X)}.
		\end{equation*}
		If $a$ satisfies the assumptions of \emph{Lax-Milgram}, we find $A \in \mathcal{L}\del[1]{L^2(X)}$, such that 
		\begin{equation*}
			a(f,\varphi) = \langle A(f),\varphi \rangle_{L^2(X)}
		\end{equation*}
		\noindent holds for all $f,\varphi \in L^2(X)$. Hence
		\begin{equation*}
			  \langle cf - g_f, \varphi \rangle_{L^2(X)} = \langle A(f),\varphi \rangle_{L^2(X)}
		\end{equation*}
		\noindent holds for all $f,\varphi \in L^2(X)$. Moreover, since $A$ is invertible, we find a unique $f_0 \in L^2(X)$, such that $A(f_0) = -u$. Therefore
		\begin{equation*}
			R_{L^2(X)}(cf_0 - g_{f_0})(\varphi) = \langle cf_0 - g_{f_0}, \varphi \rangle_{L^2(X)} = \langle -u,\varphi \rangle_{L^2(X)} = R_{L^2(X)}(-u)(\varphi)
		\end{equation*}
		\noindent holds for all $\varphi \in L^2(X)$. Thus $R_{L^2(X)}(cf_0 - g_{f_0}) = R_{L^2(X)}(-u)$ and so the \emph{Riesz representation theorem} yields that
		\begin{equation*}
			cf_0 - g_{f_0} = -u.
		\end{equation*}

		\begin{lemma}
			$a : L^2(X) \times L^2(X) \to \mathbb{C}$ is a continuous coercive sesquilinear form.
		\end{lemma}

		\begin{proof}
			Clearly $a$ is sesquilinear, i.e. antilinear in the first and linear in the second argument, by the corresponding properties of the $L^2(X)$ inner product and the simple observation that
			\begin{equation*}
				g_{f + \lambda h} = g_f + \lambda g_h
			\end{equation*}
			\noindent for $\lambda \in \mathbb{C}$ and $f,h \in L^2(X)$. Let $\varphi \in L^2(X)$. Then Cauchy-Schwarz together with lemma \ref{lem:L^2} yields
			\begin{align*}
				\abs{a(f,\varphi)} &= \abs[0]{\langle cf - g_f,\varphi \rangle_{L^2(X)}}\\
				&\leq \norm[0]{cf - g_f}_{L^2(X)}\norm[0]{\varphi}_{L^2(X)}\\
				&\leq \del[1]{c\norm[0]{f}_{L^2(X)} + \norm[0]{g_f}_{L^2(X)}}\norm{\varphi}_{L^2(X)}\\
				&\leq \del[1]{c\norm{f}_{L^2(X)} + \norm[0]{f}_{L^2(X)}\norm{L}_{L^2(X \times X)}} \norm{\varphi}_{L^2(X)}\\
				&\leq 2c\norm{f}_{L^2(X)}\norm{\varphi}_{L^2(X)} 
			\end{align*}
			\noindent since $\norm{L}_{L^2(X \times X)} < c$. Lastly, since $\norm{L}_{L^2(X \times X)} < c$, we find $c_0$ such that we have $\norm{L}_{L^2(X \times X)} < c_0 < c$ by trichotomy. Thus again lemma \ref{lem:L^2} together with Cauchy-Schwarz implies that 
			\begin{align*}
				\Re a(f,f) &= \Re \langle cf - g_f,f \rangle_{L^2(X)}\\
				&= \Re c\langle f,f \rangle_{L^2(X)} - \Re \langle g_f,f\rangle_{L^2(X)}\\
				&= c\norm{f}_{L^2(X)}^2 - \Re \langle g_f,f\rangle_{L^2(X)}\\
				&\geq c\norm{f}_{L^2(X)}^2 - \abs[0]{\langle g_f,f \rangle_{L^2(X)}}\\
				&\geq c \norm{f}_{L^2(X)}^2 - \norm[0]{g_f}_{L^2(X)}\norm{f}_{L^2(X)}\\
				&\geq c \norm{f}_{L^2(X)}^2 - \norm{f}_{L^2(X)}^2 \norm{L}_{L^2(X \times X)}\\
				&\geq (c  -c_0)\norm{f}_{L^2(X)}^2.
			\end{align*}
			Now $2c > 0$ since $c > \norm{L}_{L^2(X \times X)}$, $c - c_0 > 0$ and $c - c_0 \leq c \leq 2c$ since $c_0 > 0$.
		\end{proof}

	\item 
		~
		\begin{enumerate}[label = \textbf{\alph*.},wide = 0pt, itemsep = 1.5ex]
			\item Suppose that $M \setminus \wbar{A}$ is dense in $M$. Towards a contradiction, assume that $A$ is not nowhere dense. Hence $\mathring{\wbar{A}} \neq \varnothing$. Since $\mathring{\wbar{A}}$ is open by definition of the interior of a set, there exists $\varepsilon > 0$ and $x \in \mathring{\wbar{A}}$ such that $B_\varepsilon(x) \subseteq \mathring{\wbar{A}}$. Moreover, $\mathring{\wbar{A}} \subseteq \wbar{A}$ and thus $B_\varepsilon(x) \subseteq \wbar{A}$. This implies that $B_\varepsilon(x)$ and $M \setminus \wbar{A}$ are disjoint. But $M \setminus \wbar{A}$ is dense in $M$, hence we find a sequence $(x_n)_{n \in \mathbb{N}}$ in $M \setminus \wbar{A}$ such that $x_n \to x$. Hence there exists $N \in \mathbb{N}$ such that $x_n \in B_\varepsilon(x)$ for all $n \geq N$. This is not possible since $B_\varepsilon(x)$ does not contain any elements of $M \setminus \wbar{A}$. Contradiction. 

			\item 
				\begin{lemma}
					Let $(x_k)_{k \in \mathbb{N}}$ be an enumeration of $\mathbb{Q}$. For $n \in \mathbb{N}$ define
					\begin{equation}
						E_n := \bigcup_{k \in \mathbb{N}} \intoo[3]{x_k - \frac{1}{2^kn},x_k + \frac{1}{2^kn}}
					\end{equation}
					\noindent and
					\begin{equation}
						E := \bigcap_{n \in \mathbb{N}} E_n.
					\end{equation}
					Set $A := E^c$. Then $A$ is meager and $\lambda(A^c) = 0$, where $\lambda$ denotes the ordinary Lebesgue measure on $\mathbb{R}$. 
				\end{lemma}

				\begin{proof}
					We show first that $\lambda(A^c) = 0$. First observe that $(E_n)_{n \in \mathbb{N}}$ is a decreasing sequence of $\lambda$-measurable sets. Moreover, for any $n \in \mathbb{N}$ we have that 
					\begin{equation*}
						\lambda(E_n) \leq \frac{1}{n}\sum_{k \in \mathbb{N}}\frac{1}{2^{k-1}} = \frac{1}{n}\sum_{k \in \mathbb{N}_0}\frac{1}{2^{k}} = \frac{2}{n} < \infty 
					\end{equation*}
					\noindent by subadditivity of the measure. Elementary measure theory now tells us that
					\begin{equation*}
						\lambda(A^c) = \lambda(E) = \lambda\del[1]{\cap_{n \in \mathbb{N}} E_n} = \lim_{n \to \infty}\lambda(E_n) \leq \lim_{n \to \infty} \frac{2}{n} = 0. 	
					\end{equation*}
					Let us show that $A$ is meager. Since $A = E^c = \cup_{n \in \mathbb{N}} E_n^c$, we show that $E_n^c$ is nowhere dense for all $n \in \mathbb{N}$. By part \textbf{a.} we can also show that $\mathbb{R} \setminus \wbar{E_n^c}$ is dense in $\mathbb{R}$. For fixed $n \in \mathbb{N}$ we have that
					\begin{equation*}
						E_n^c = \bigcap_{k \in \mathbb{N}}\del[3]{\intoc[2]{-\infty, x_k - \frac{1}{2^kn}} \cup \intco[2]{x_k + \frac{1}{2^kn},\infty}}.
					\end{equation*}
					Thus $E_n^c$ is a closed set (finite unions and countable intersection of closed intervals) and so $\wbar{E_n^c} = E_n^c$. So $\mathbb{R} \setminus \wbar{E_n^c} = E_n$. But $\mathbb{Q} \subseteq E_n$ for all $n \in \mathbb{N}$ and thus $E_n$ is dense in $\mathbb{R}$.
				\end{proof}
		\end{enumerate}
	\item
		~
		\begin{enumerate}[label = \textbf{\alph*.},wide = 0pt, itemsep = 1.5ex]
			\item If $A = \varnothing$, we have that $\cap_{\alpha \in A} \mathcal{T}_\alpha = \mathcal{P}(X)$ since topologies on $X$ are subsets of $\mathcal{P}(X)$. Hence the intersection of the empty family of topologies on $X$ is the discrete topology.\\
				Consider now $A \neq \varnothing$. Clearly, $\varnothing, X \in \cap_{\alpha \in A} \mathcal{T}_\alpha$ since $\varnothing,X \in \mathcal{T}_{\alpha}$ for all $\alpha \in A$. Let $U_1,\dots,U_n \in \cap_{\alpha \in A}\mathcal{T}_\alpha$. Hence $U_1,\dots,U_n \in \mathcal{T}_\alpha$ for all $\alpha \in A$ and so $U_1 \cap \dots \cap U_n \in \mathcal{T}_\alpha$ for all $\alpha \in A$. Hence $U_1 \cap \dots \cap U_n \in \cap_{\alpha \in A}\mathcal{T}_\alpha$. Finally, suppose that $(U_\beta)_{\beta \in B}$ is a family in $\cap_{\alpha \in A} \mathcal{T}_\alpha$. Hence for all $\alpha \in A$ we have that $U_\beta \in \mathcal{T}_\alpha$ for all $\beta \in B$. So $\cup_{\beta \in B} U_\beta \in \mathcal{T}_\alpha$ for all $\alpha \in A$ and therefore $\cup_{\beta \in B} U_\beta \in \cap_{\alpha \in A} \mathcal{T}_\alpha$.
			\item Define
				\begin{equation*}
					\mathcal{B} := \cbr{U_1 \cap \dots \cap U_n : n \in \mathbb{N},U_i \in \mathcal{\altS} \text{ for all } i = 1,\dots,n}
				\end{equation*}
				\noindent and 
				\begin{equation*}
					\mathcal{T} := \cbr{\textstyle{\cup}_{\alpha \in A} B_\alpha : B_\alpha \in A \text{ for all } \alpha \in A}.
				\end{equation*}
		
				\begin{lemma}
					$\mathcal{T}_\mathcal{F} = \mathcal{T}$.
				\end{lemma}

				\begin{proof}
					By part \textbf{a.}, $\mathcal{T}_\mathcal{F}$ is a topology. We show that also $\mathcal{T}$ is a topology. By \cite[34]{lee:topological_manifolds:2011} it is enough to show that $\mathcal{B}$ satisfies the following two conditions:
					\begin{enumerate}[label = (\roman*)]
						\item $\cup_{B \in \mathcal{B}} B = X$.
						\item If $B_1,B_2 \in \mathcal{B}$ and $x \in B_1 \cap B_2$, there exists an element $B_3 \in \mathcal{B}$ such that $x \in B_3 \subseteq B_1 \cap B_2$.
					\end{enumerate}
					Then $\mathcal{T}$ is the unique topology on $X$ generated by $\mathcal{B}$, i.e. the collection of arbitrary unions of elements of $\mathcal{B}$. Since $\mathcal{F}$ is nonempty, there exists $f \in \mathcal{F}$. Clearly $X = f^{-1}(Y_f)$ and $Y_f$ is open in $Y_f$. Hence $f^{-1}(Y_f) \in \mathcal{\altS}$ and thus $X \in \cup_{B \in \mathcal{B}} B$. Suppose that $B_1,B_2 \in \mathcal{B}$ such that $B_1 \cap B_2 \neq \varnothing$. Hence we find $U_1,\dots,U_n,V_1,\dots,V_m \in \mathcal{\altS}$ such that $B_1 = U_1 \cap \dots \cap U_n$ and $B_2 = V_1 \cap \dots \cap V_m$. Suppose $x \in B_1 \cap B_2$. Then also $x \in U_1 \cap \dots \cap U_n \cap V_1 \cap \dots \cap V_m$. But 
					\begin{equation*}
						U_1 \cap \dots \cap U_n \cap V_1 \cap \dots \cap V_m \in \mathcal{B}
					\end{equation*}
					\noindent as a finite intersection of elements of $\mathcal{\altS}$. Hence $\mathcal{T}$ is a topology.\\
					Clearly, $\mathcal{\altS} \subseteq \mathcal{T}$, since already $\mathcal{\altS} \subseteq \mathcal{B}$. Since $\mathcal{T}_\mathcal{F}$ is the smallest topology containing $\mathcal{\altS}$, we get that $\mathcal{T}_\mathcal{F} \subseteq \mathcal{T}$.\\
					Let $U \in \mathcal{T}$. Then $U = \cup_{\alpha \in A}B_\alpha$ for some index set $A$ and $B_\alpha \in \mathcal{B}$ for all $\alpha \in A$. But each $B_\alpha$ is a finite intersection of elements of $\mathcal{\altS}$ and thus since $\mathcal{T}_\mathcal{F}$ is a topology containing $\mathcal{\altS}$, we have that $B_\alpha \in \mathcal{T}_\mathcal{F}$ for all $\alpha \in A$. But then also $U \in \mathcal{T}_\mathcal{F}$ as a union of sets in $\mathcal{T}_\mathcal{F}$. Hence $\mathcal{T} \subseteq \mathcal{T}_\mathcal{F}$. 
				\end{proof}
		\end{enumerate}
	\item Suppose that $x_n \rightharpoonup x$. Proposition 6.2.2 implies that the sequence $(x_n)_{n \in \mathbb{N}}$ is bounded, in particular $\sup_{n \in \mathbb{N}} \norm{x_n} < \infty$. Moreover, lemma 6.2.1 yields $f(x_n) \to f(x)$ for all $f \in X^*$. Since $Y \subseteq X^*$ we also have $f(x_n) \to f(x)$ for all $f \in Y$.\\
		Conversly, suppose $\norm{x_n} \leq M$ for some $M \geq 0$ and $f(x_n) \to f(x)$ for all $f \in Y$. Let $f \in X^*$. Since $Y$ is dense in $X^*$, we find a sequence $(f_k)_{k \in \mathbb{N}}$ in $Y$ such that $\norm{f_k - f} \to 0$. Hence
		\begin{align*}
			\abs{f(x_n) - f(x)} &= \abs{f(x_n) - f(x) + f_k(x_n) - f_k(x_n) + f_k(x) - f_k(x)}\\
			&\leq \abs{f(x_n) - f_k(x_n)} + \abs{f_k(x_n) - f_k(x)} + \abs{f_k(x) - f(x)}\\
			&\leq \norm{f - f_k}\del[0]{\norm{x_n} + \norm{x}} + \abs{f_k(x_n) - f_k(x)}\\
			&\leq \norm{f - f_k}\del[0]{M + \norm{x}} + \abs{f_k(x_n) - f_k(x)}\\
		\end{align*}
		\noindent and so
		\begin{equation*}
			\lim_{n \to \infty} \abs{f(x_n) - f(x)} \leq \norm{f - f_k}\del[0]{M + \norm{x}} \xrightarrow{k \to \infty} 0.
		\end{equation*}
		Thus $f(x_n) \to f(x)$ for all $f \in X^*$ and so lemma 6.2.1 implies $x_n \rightharpoonup x$.
\end{enumerate}
\printbibliography
\end{document}
